code/experimental/P256/Hacl.Spec.P256.fst
@@ -8,6 +8,7 @@ open Lib.ByteSequence
 open Lib.IntTypes
 open Lib.Sequence
 
+#reset-options " --z3rlimit 100" 
 
 let prime = prime256
 noextract
@@ -87,10 +88,10 @@ let _norm (p:point_nat): (point_nat) =
   let z3 = z * z * z in 
   let z3i = modp_inv2_pow z3 in 
   let x3 = (z2i * x) % prime256 in 
-  let y3 = (z3i * y) % prime256 in 
+  let y3 = (z3i * y) % prime256 in  
   let z3 = if isPointAtInfinity p then 0 else 1 in 
-  assert(x3 == (x * (pow (z * z) (prime256 -2) % prime256) % prime256));
-  assert(y3 == (y * (pow (z * z * z) (prime256 - 2) % prime256) % prime256));
+  assert(x3 == (x * (pow (z * z) (prime256 - 1) % prime256) % prime256));
+  assert(y3 == (y * (pow (z * z * z) (prime256 - 1) % prime256) % prime256));
   (x3, y3, z3)
 
 
